{
 "cells": [
  {
   "cell_type": "markdown",
   "metadata": {},
   "source": [
    "#### 3. We empirically demonstrated convergence to the mean for the toss of a coin. Calculate the variance of the estimate of the probability that we see a head after drawing $n$ samples."
   ]
  },
  {
   "cell_type": "markdown",
   "metadata": {},
   "source": [
    "Let $X_i \\in \\{0, 1\\}$ denote if the $i$th flip landed on head and consider \n",
    "$$\n",
    "\\tilde{X}_n := \\sum_{i = 1}^n X_i.\n",
    "$$\n",
    "We are interested in $P(\\tilde{X}_n \\geq 1)$. Note that for $k \\in {0, \\dots, n}$ the statement $\\tilde{X}_n = k$ is equivalent to there being exactly $k$ heads, which means we have $k$ heads and $n - k$ tails. Denote by $p$ the probability of getting heads, then flipping $k$ heads and $n - k$ tails has a probability of\n",
    "$$\n",
    "p^k (1 - p)^{n - k}\n",
    "$$\n",
    "and because the order of those doesn't matter we have to multiply this with the number of permutations, i.e., we are interested in how many arrangements there are to distribute $k$ (or equivalently $n - k$) elements in $n$ slots. This is exactly the binomial coefficient\n",
    "$$\n",
    "\\binom{n}{k} = \\frac{n!}{k! (n - k)!}.\n",
    "$$\n",
    "In total this means\n",
    "$$\n",
    "P(\\tilde{X}_n = k) = \\binom{n}{k} p^k (1 - p)^{n - k}.\n",
    "$$\n",
    "\n",
    "Looking back on it now, I just realized that the $X_i$ are all independent as such\n",
    "$$\n",
    "E[\\tilde{X}_n] = E\\left[\\sum_{i = 1}^n X_i\\right] = \\sum_{i = 1}^n E[X_i] = \\sum_{i = 1}^n p = np.\n",
    "$$\n",
    "\n",
    "Alternatively the expected value of $\\tilde{X}_n$ can then be calculated directly as\n",
    "$$\n",
    "\\begin{aligned}\n",
    "E[\\tilde{X}_n] &= \\sum_{k = 0}^n kP(\\tilde{X}_n = k) \\\\\n",
    "&= \\sum_{k = 0}^n k \\binom{n}{k} p^k (1 - p)^{n - k} \\\\\n",
    "&= \\sum_{k = 0}^n k \\binom{n}{k} p^k (1 - p)^{n - k}.\n",
    "\\end{aligned}\n",
    "$$\n",
    "This can be explicitly calculated to be $np$, we're only going to prove the case where $p = 1 - p = 0.5$, in that case\n",
    "$$\n",
    "\\begin{aligned}\n",
    "E[\\tilde{X}_n] &= \\sum_{k = 0}^n k \\binom{n}{k} 2^{-n}\n",
    "&= 2^{-n} \\sum_{k = 0}^n k \\binom{n}{k} \\\\\n",
    "&\\overset{*}{=} 2^{-n} 2^{n - 1} = n / 2 = pn.\n",
    "\\end{aligned}\n",
    "$$\n",
    "What remains to be shown is that $(*)$ holds. This can be done inductively, it obviously holds for $n = 1$. Now suppose the identity holds for some $n \\in \\mathbb{N}$, then\n",
    "$$\n",
    "\\sum_{k = 0}^{n + 1} k \\binom{n + 1}{k} = (n + 1) + \\sum_{k = 0}^n k \\binom{n + 1}{k},\n",
    "$$\n",
    "using Pascal's triangle equality we can write\n",
    "$$\n",
    "\\binom{n + 1}{k} = \\binom{n}{k} + \\binom{n}{k - 1}.\n",
    "$$\n",
    "With this we can then calculate\n",
    "$$\n",
    "\\begin{aligned}\n",
    "\\sum_{k = 0}^{n + 1} k \\binom{n + 1}{k} &= (n + 1) + \\sum_{k = 0}^n k \\binom{n + 1}{k} \\\\\n",
    "&= (n + 1) + \\sum_{k = 0}^n k \\left[ \\binom{n}{k} + \\binom{n}{k - 1} \\right] \\\\\n",
    "&= (n + 1) + \\sum_{k = 0}^n k \\binom{n}{k} + \\sum_{k = 0}^n k \\binom{n}{k - 1} \\\\\n",
    "&= (n + 1) + \\sum_{k = 0}^n k \\binom{n}{k} + \\sum_{k = 0}^{n - 1} (k + 1) \\binom{n}{k} \\\\\n",
    "&= (n + 1) + \\sum_{k = 0}^n k \\binom{n}{k} + \\sum_{k = 0}^{n - 1} k \\binom{n}{k} + \\sum_{k = 0}^{n - 1} \\binom{n}{k} \\\\\n",
    "&= (n + 1) + \\sum_{k = 0}^n k \\binom{n}{k} + \\sum_{k = 0}^n k \\binom{n}{k} + \\sum_{k = 0}^{n - 1} \\binom{n}{k} - n \\\\\n",
    "&= 2 \\sum_{k = 0}^n k \\binom{n}{k} - n + \\sum_{k = 0}^n \\binom{n}{k} - 1.\n",
    "\\end{aligned}\n",
    "$$\n",
    "Applying the well-known identity\n",
    "$$\n",
    "\\sum_{k = 0}^n \\binom{n}{k} = 2^n\n",
    "$$\n",
    "and the induction hypothesis to this yields\n",
    "$$\n",
    "2 (2^{n - 1}) + 2^n = 2^{n + 1}.\n",
    "$$\n",
    "By induction it then follows that for all $n \\in \\mathbb{N}$ the identity\n",
    "$$\n",
    "\\sum_{k = 0}^n k \\binom{n}{k} = 2^n\n",
    "$$\n",
    "holds.\n",
    "\n",
    "Just as for the expected value\n",
    "$$\n",
    "\\operatorname{Var}[\\tilde{X}_n] = \\sum_{i = 1}^n \\operatorname{Var}[X_i] = np(1 - p).\n",
    "$$"
   ]
  },
  {
   "cell_type": "markdown",
   "metadata": {},
   "source": []
  }
 ],
 "metadata": {
  "language_info": {
   "name": "python"
  }
 },
 "nbformat": 4,
 "nbformat_minor": 2
}
