{
 "cells": [
  {
   "cell_type": "markdown",
   "metadata": {},
   "source": [
    "#### 1. Prove that the transpose of the transpose of a matrix is the matrix itself:"
   ]
  },
  {
   "cell_type": "markdown",
   "metadata": {},
   "source": [
    "The transpose per definition satisfies $(A^T)_{ij} = A_{ji}$ for all $i, j$. As such $((A^T)^T)_{ij} = (A^T)_{ji} = A_{ij}$, which shows that $(A^T)^T = A$."
   ]
  }
 ],
 "metadata": {
  "language_info": {
   "name": "python"
  }
 },
 "nbformat": 4,
 "nbformat_minor": 2
}
